refinement update

refinement.v
@@ -18,7 +18,7 @@ Inductive refineone : SimpleUML -> SimpleUML -> Prop :=
     not (set_In c' C) -> 
     set_In ci C ->
     let C' := (c':: C) in
-    let G' := set_add eqGen_dec (BGen ci c') G in 
+    let G' := (BGen ci c') :: G in 
     refineone (mkSimpleUML C T P S G) (mkSimpleUML C' T P S G')
 | dec2 : forall c' ci C T P S G,
     not (set_In c' C) ->
@@ -45,3 +45,56 @@ Inductive refineone : SimpleUML -> SimpleUML -> Prop :=
     let S' := (CA c' ci directed) :: S in
     refineone (mkSimpleUML C T P S G) (mkSimpleUML C' T P S' G)
 .
+
+
+Inductive refine : SimpleUML -> SimpleUML -> Prop :=
+| one : forall m1 m2, refineone m1 m2 -> refine m1 m2
+| reflex : forall m, refine m m
+| trans : forall m1 m2 m3, refine m1 m2 -> refine m2 m3 -> refine m1 m3
+.
+
+Theorem wellFormed_preserve :
+  forall m1 m2, WellFormed m1 -> refineone m1 m2 ->
+           WellFormed m2.
+Proof.
+  intros m1 m2 H1 H2.
+  inversion H1. unfold UniqueClass in H.
+  inversion H2; subst; simpl in H.
+Admitted.
+
+Theorem refine_refl :
+  forall m, refine m m.
+Proof.
+  intros m. apply reflex.
+Qed.
+
+
+Theorem refine_trans :
+  forall m1 m2 m3, refine m1 m2 -> refine m2 m3
+              -> refine m1 m3.
+Proof.
+  intros m1 m2 m3 H1 H2.
+  apply trans with m2; assumption.
+Qed.
+
+
+Theorem class_preserve :
+  forall c m1 m2, refineone m1 m2 ->
+             set_In c (MClass_Instance m1) ->
+             set_In c (MClass_Instance m2).
+Proof.
+  intros c m1 m2 H.
+  induction H; intros H1; simpl;
+    simpl in H1; right; assumption.
+Qed.
+
+
+Theorem gen_preserve :
+  forall sub super m1 m2, refineone m1 m2 ->
+                     set_In (BGen super sub) (MGen_Instance m1) ->
+                     set_In (BGen super sub) (MGen_Instance m2).
+Proof.
+  intros sub super m1 m2 H.
+  induction H; intros H1; simpl in H1; simpl; try assumption.
+  - right; assumption.
+Qed.
